{
 "cells": [
  {
   "cell_type": "markdown",
   "metadata": {},
   "source": [
    "# Derivatives\n",
    "\n",
    "\n",
    "### Derivative of a constant function\n",
    "\n",
    "The derivative of f(x) = c where c is a constant is given by\n",
    "\n",
    "$ f^\\prime (x) = 0 $\n",
    "\n",
    "**Example**\n",
    "\n",
    "$ f(x) = -10 $, then $ f^\\prime (x) = 0 $\n",
    "\n",
    "### Derivative of the power of two functions (Power Rule)\n",
    "\n",
    "The derivative of a power function. The derivative of $f(x) = x^r$ where r is a constant real number is\n",
    "\n",
    "$ f^\\prime(x) = r x^{r-1}$\n",
    "\n",
    "**Example**\n",
    "\n",
    "$ f(x) = x^{-2}$, then $ f^\\prime(x) = -2 x ^{-3} = \\frac{-2}{x^{3}} $\n",
    "\n",
    "### Derivative of a function multiplied by a constant\n",
    "\n",
    "The derivative of f(x) = cg(x) is given by\n",
    "\n",
    "$ f^\\prime{x} = cg^{\\prime}(x) $\n",
    "\n",
    "**Example**\n",
    "\n",
    "$ f(x) = 3x^3$\n",
    "let c = 3 and $g(x) = x^3$, then $ f^\\prime(x) = cg^\\prime(x) $\n",
    "\n",
    "$ = 3(3x^2) = 9x^2 $\n",
    "\n",
    "### Derivative of the sum of functions (Sum Rule) \n",
    "\n",
    "The derivative of $f(x) = g(x) + h(x)$ is given by\n",
    "\n",
    "$ f^\\prime(x) = g^\\prime(x) + h^\\prime(x) $\n",
    "\n",
    "**Example**\n",
    "\n",
    "$ f(x) = x^2 + 4 $\n",
    "\n",
    "let $g(x) = x^2$ and $h(x) = 4$, then $f^\\prime(x) = g^\\prime(x) + h^\\prime(x) = 2(x) + 0 = 2x$\n",
    "\n",
    "### Derivative of the difference of functions\n",
    "\n",
    "The derivative of $f(x) = g(x) - h(x) $ is given by\n",
    "\n",
    "$ f^\\prime(x) = g^\\prime(x) - h^\\prime(x) $\n",
    "\n",
    "**Example**\n",
    "\n",
    "$f(x) = x^3 - x^{-2} $\n",
    "\n",
    "let $g(x) = x^3$ and $h(x) = x^{-2}$, then\n",
    "\n",
    "$ f^\\prime(x) = g^\\prime(x) - h^\\prime(x) = 3x^2 - (-2x^{-3}) = 3x^2 + 2x^{-3} $\n",
    "\n",
    "### Derivative of the product of two functions (Product Rule)\n",
    "\n",
    "The derivative of $f(x) = g(x) h(x)$ is given by\n",
    "\n",
    "$ f^\\prime(x) = g(x) h^\\prime(x) + h(x) g^\\prime(x) $\n",
    "\n",
    "**Example**\n",
    "\n",
    "$ f(x) = (x^2 - 2x) (x-2) $ \n",
    "\n",
    "let $g(x) = (x^2 - 2x)$ and $h(x) = (x - 2)$, then\n",
    "\n",
    "$f^\\prime(x) = g(x)h^\\prime(x) + h(x)g^\\prime(x) = (x^2 - 2x)(1) + (x-2)(2x-2) $\n",
    "\n",
    "$= x^2 - 2x + 2x^2 - 6x + 4 = 3x^2 - 8x + 4$\n",
    "\n",
    "### Derivative of the quotient of two functions (Quotient Rule)\n",
    "\n",
    "The derivative of f(x) = g(x) / h(x) is given by\n",
    "\n",
    "$$ f^\\prime(x) = \\frac{(h(x)g^\\prime(x) - g(x)h^\\prime(x))}{h(x)^2} $$\n",
    "\n",
    "**Example**\n",
    "\n",
    "$f(x) = \\frac{(x-2)}{(x+1)} $\n",
    "\n",
    "let $g(x) = (x-2) $ and $h(x) = (x+1)$, then\n",
    "\n",
    "$$f^\\prime(x) = \\frac{(h(x)g^\\prime(x) - g(x)h^\\prime(x))}{h(x)^2}$$\n",
    "\n",
    "$$ = \\frac{(x+1)(1) - (x-2)(1)}{(x+1)^2} $$\n",
    "\n",
    "$$ = \\frac{3}{(x+1)^2} $$"
   ]
  },
  {
   "cell_type": "code",
   "execution_count": null,
   "metadata": {
    "collapsed": true
   },
   "outputs": [],
   "source": []
  }
 ],
 "metadata": {
  "kernelspec": {
   "display_name": "Python 3",
   "language": "python",
   "name": "python3"
  },
  "language_info": {
   "codemirror_mode": {
    "name": "ipython",
    "version": 3
   },
   "file_extension": ".py",
   "mimetype": "text/x-python",
   "name": "python",
   "nbconvert_exporter": "python",
   "pygments_lexer": "ipython3",
   "version": "3.6.8"
  }
 },
 "nbformat": 4,
 "nbformat_minor": 2
}
